
\section{Question}

\paragraph{Q1}


f0(a,b,c,d)= $[5, 7, 13, 15]$
f1(a,b,c,d)= $[6, 7, 9, 11, 13, 14]$
f2(a,b,c,d)= $[10, 11, 14]$
f3(a,b,c,d)= $[15]$

\hrule width 1\linewidth
\paragraph{Q1}


f0(a,b,c,d)= $[5, 7, 13, 15]$
f1(a,b,c,d)= $[6, 7, 9, 11, 13, 14]$
f2(a,b,c,d)= $[10, 11, 14]$
f3(a,b,c,d)= $[15]$

\hrule width 1\linewidth
\paragraph{Q1}


f0(a,b,c,d)= $[5, 7, 13, 15]$
f1(a,b,c,d)= $[6, 7, 9, 11, 13, 14]$
f2(a,b,c,d)= $[10, 11, 14]$
f3(a,b,c,d)= $[15]$

\hrule width 1\linewidth
\paragraph{Q1}


f0(a,b,c,d)= $[5, 7, 13, 15]$
f1(a,b,c,d)= $[6, 7, 9, 11, 13, 14]$
f2(a,b,c,d)= $[10, 11, 14]$
f3(a,b,c,d)= $[15]$

\hrule width 1\linewidth
\paragraph{Q1}


f0(a,b,c,d)= $[5, 7, 13, 15]$
f1(a,b,c,d)= $[6, 7, 9, 11, 13, 14]$
f2(a,b,c,d)= $[10, 11, 14]$
f3(a,b,c,d)= $[15]$

\hrule width 1\linewidth
\paragraph{Q1}


f0(a,b,c,d)= $[5, 7, 13, 15]$
f1(a,b,c,d)= $[6, 7, 9, 11, 13, 14]$
f2(a,b,c,d)= $[10, 11, 14]$
f3(a,b,c,d)= $[15]$

\hrule width 1\linewidth\pagebreak
\subsection{Correction}

\paragraph{Q1}

%\begin{table}
        \begin{tabular}{|c|c|c|c|c||c|c|c|c|}
    \toprule
         & A & B & C & D & S0 & S1 & S2 & S3\\ \midrule0 & 0 & 0 & 0 & 0 & 0 & 0 & 0 & 0\\1 & 0 & 0 & 0 & 1 & 0 & 0 & 0 & 0\\2 & 0 & 0 & 1 & 0 & 0 & 0 & 0 & 0\\3 & 0 & 0 & 1 & 1 & 0 & 0 & 0 & 0\\\midrule4 & 0 & 1 & 0 & 0 & 0 & 0 & 0 & 0\\5 & 0 & 1 & 0 & 1 & 1 & 0 & 0 & 0\\6 & 0 & 1 & 1 & 0 & 0 & 1 & 0 & 0\\7 & 0 & 1 & 1 & 1 & 1 & 1 & 0 & 0\\\midrule8 & 1 & 0 & 0 & 0 & 0 & 0 & 0 & 0\\9 & 1 & 0 & 0 & 1 & 0 & 1 & 0 & 0\\10 & 1 & 0 & 1 & 0 & 0 & 0 & 1 & 0\\11 & 1 & 0 & 1 & 1 & 0 & 1 & 1 & 0\\\midrule12 & 1 & 1 & 0 & 0 & 0 & 0 & 0 & 0\\13 & 1 & 1 & 0 & 1 & 1 & 1 & 0 & 0\\14 & 1 & 1 & 1 & 0 & 0 & 1 & 1 & 0\\15 & 1 & 1 & 1 & 1 & 1 & 0 & 0 & 1\\\bottomrule
        \end{tabular}
        %%\end{table}
        f0(a,b,c,d)=$[5, 7, 13, 15]$

f0(a,b,c,D)=$ \sum [5, 7, 13, 15] $ 


Sum of products 
 f0(a,b,c,d) = $\bar a.\bar b.\bar c.d + \bar a.\bar b.\bar c.d + \bar a.\bar b.\bar c.d + \bar a.\bar b.\bar c.d$

Product of sums 
 f0(a,b,c,d) = $a.b.c.d.\bar a.\bar b.\bar c.\bar d.\bar a.\bar b.\bar c.d.\bar a.\bar b.\bar c.\bar d.\bar a.\bar b.c.d.\bar a.\bar b.\bar c.d.\bar a.b.c.d.\bar a.\bar b.\bar c.\bar d.\bar a.\bar b.\bar c.d.\bar a.\bar b.\bar c.\bar d.\bar a.\bar b.c.d.\bar a.\bar b.\bar c.d$
f1(a,b,c,d)=$[6, 7, 9, 11, 13, 14]$

f1(a,b,c,D)=$ \sum [6, 7, 9, 11, 13, 14] $ 


Sum of products 
 f1(a,b,c,d) = $\bar a.\bar b.c.\bar d + \bar a.\bar b.\bar c.d + \bar a.\bar b.\bar c.d + \bar a.\bar b.\bar c.d + \bar a.\bar b.\bar c.d + \bar a.\bar b.c.\bar d$

Product of sums 
 f1(a,b,c,d) = $a.b.c.d.\bar a.\bar b.\bar c.\bar d.\bar a.\bar b.\bar c.d.\bar a.\bar b.\bar c.\bar d.\bar a.\bar b.c.d.\bar a.\bar b.\bar c.\bar d.\bar a.b.c.d.\bar a.\bar b.\bar c.d.\bar a.\bar b.c.d.\bar a.\bar b.\bar c.\bar d$
f2(a,b,c,d)=$[10, 11, 14]$

f2(a,b,c,D)=$ \sum [10, 11, 14] $ 


Sum of products 
 f2(a,b,c,d) = $\bar a.\bar b.c.\bar d + \bar a.\bar b.\bar c.d + \bar a.\bar b.c.\bar d$

Product of sums 
 f2(a,b,c,d) = $a.b.c.d.\bar a.\bar b.\bar c.\bar d.\bar a.\bar b.\bar c.d.\bar a.\bar b.\bar c.\bar d.\bar a.\bar b.c.d.\bar a.\bar b.\bar c.\bar d.\bar a.\bar b.\bar c.d.\bar a.\bar b.\bar c.\bar d.\bar a.b.c.d.\bar a.\bar b.\bar c.\bar d.\bar a.\bar b.c.d.\bar a.\bar b.\bar c.\bar d.\bar a.\bar b.\bar c.\bar d$
f3(a,b,c,d)=$[15]$

f3(a,b,c,D)=$ \sum [15] $ 


Sum of products 
 f3(a,b,c,d) = $\bar a.\bar b.\bar c.d$

Product of sums 
 f3(a,b,c,d) = $a.b.c.d.\bar a.\bar b.\bar c.\bar d.\bar a.\bar b.\bar c.d.\bar a.\bar b.\bar c.\bar d.\bar a.\bar b.c.d.\bar a.\bar b.\bar c.\bar d.\bar a.\bar b.\bar c.d.\bar a.\bar b.\bar c.\bar d.\bar a.b.c.d.\bar a.\bar b.\bar c.\bar d.\bar a.\bar b.\bar c.d.\bar a.\bar b.\bar c.\bar d.\bar a.\bar b.c.d.\bar a.\bar b.\bar c.\bar d.\bar a.\bar b.\bar c.d$

Karnough map\todo{fix map}
\begin{karnaugh-map}[4][4][1][cd][ab]
          \minterms{5, 7, 13, 15}
          \maxterms{0, 1, 2, 3, 4, 6, 8, 9, 10, 11, 12, 14}
        %\autoterms[0]
          %\implicant{5}{15}
          %\implicantedge{8}{8}{10}{10}
          %\implicantedge{8}{8}{10}{10}[8,10]
        \end{karnaugh-map}

Simplified Sum of products f0 : $b.d$

Simplified Product of sums f0: $b.d$

Karnough map\todo{fix map}
\begin{karnaugh-map}[4][4][1][cd][ab]
          \minterms{6, 7, 9, 11, 13, 14}
          \maxterms{0, 1, 2, 3, 4, 5, 8, 10, 12, 15}
        %\autoterms[0]
          %\implicant{5}{15}
          %\implicantedge{8}{8}{10}{10}
          %\implicantedge{8}{8}{10}{10}[8,10]
        \end{karnaugh-map}

Simplified Sum of products f1 : $a.\bar b.d+a.\bar c.d+\bar a.b.c+b.c.\bar d$

Simplified Product of sums f1: $(a+\bar b+b).(a+\bar c+c).(b+\bar d)+d).(\bar a+d).(c$

Karnough map\todo{fix map}
\begin{karnaugh-map}[4][4][1][cd][ab]
          \minterms{10, 11, 14}
          \maxterms{0, 1, 2, 3, 4, 5, 6, 7, 8, 9, 12, 13, 15}
        %\autoterms[0]
          %\implicant{5}{15}
          %\implicantedge{8}{8}{10}{10}
          %\implicantedge{8}{8}{10}{10}[8,10]
        \end{karnaugh-map}

Simplified Sum of products f2 : $a.\bar b.c+a.c.\bar d$

Simplified Product of sums f2: $a.c.(\bar b+\bar d)$

Karnough map\todo{fix map}
\begin{karnaugh-map}[4][4][1][cd][ab]
          \minterms{15}
          \maxterms{0, 1, 2, 3, 4, 5, 6, 7, 8, 9, 10, 11, 12, 13, 14}
        %\autoterms[0]
          %\implicant{5}{15}
          %\implicantedge{8}{8}{10}{10}
          %\implicantedge{8}{8}{10}{10}[8,10]
        \end{karnaugh-map}

Simplified Sum of products f3 : $a.b.c.d$

Simplified Product of sums f3: $a.b.c.d$
\paragraph{Logigramme} de la fonction\\
            %%\missingfigure[figwidth=6cm]{Logigramme}

 \begin{tikzpicture}

\node (x) at (0, 1*1.5) {$A$};
            \node (y) at (0.5, 1*1.5) {$B$};
            \node (z) at (1, 1*1.5) {$C$};
            \node (w) at (1.5, 1*1.5) {$D$};
            \node[not gate US, draw, rotate=270] at ($(x) + (0.25, -0.3)$) (notx) {};
            \draw (x) -- (notx.input); 
            \node[not gate US, draw, rotate=270] at ($(y) + (0.25, -0.3)$) (noty) {};
            \draw (y) -- (noty.input); 
            \node[not gate US, draw, rotate=270] at ($(z) + (0.25, -0.3)$) (notz) {};
            \draw (z) -- (notz.input);
            \node[not gate US, draw, rotate=270] at ($(w) + (0.25, -0.3)$) (notw) {};
            \draw (w) -- (notw.input);
                
           
            \node[and gate US, draw, rotate=0, logic gate inputs=nnnn] at (2.5, 0*1.5) (xandy0) {};
            \draw (xandy0.output) -- node[above]{\scriptsize $B.D$} ($(xandy0) + (1.8, 0)$);
              
            %% Y
            \draw (y) -| ($(y) + (0, 0)$) |- (xandy0.input 2);
            %%W
            \draw (w) -| ($(w) + (0, 0)$) |- (xandy0.input 4);
        \node[or gate US, draw, rotate=0, logic gate inputs=nn] at (5.5, 1*0.5) (xory) {};


                    \draw (xory.output) -- node[above]{\scriptsize$F$} ($(xory) + (1, 0)$);

\draw (xandy0.output) -- ([xshift=1.40cm]xandy0.output) |- (xory.input 1);

 \end{tikzpicture}

\paragraph{Logigramme} de la fonction\\
            %%\missingfigure[figwidth=6cm]{Logigramme}

 \begin{tikzpicture}

\node (x) at (0, 4*1.5) {$A$};
            \node (y) at (0.5, 4*1.5) {$B$};
            \node (z) at (1, 4*1.5) {$C$};
            \node (w) at (1.5, 4*1.5) {$D$};
            \node[not gate US, draw, rotate=270] at ($(x) + (0.25, -0.3)$) (notx) {};
            \draw (x) -- (notx.input); 
            \node[not gate US, draw, rotate=270] at ($(y) + (0.25, -0.3)$) (noty) {};
            \draw (y) -- (noty.input); 
            \node[not gate US, draw, rotate=270] at ($(z) + (0.25, -0.3)$) (notz) {};
            \draw (z) -- (notz.input);
            \node[not gate US, draw, rotate=270] at ($(w) + (0.25, -0.3)$) (notw) {};
            \draw (w) -- (notw.input);
                
           
            \node[and gate US, draw, rotate=0, logic gate inputs=nnnn] at (2.5, 0*1.5) (xandy0) {};
            \draw (xandy0.output) -- node[above]{\scriptsize $A.\bar B.D$} ($(xandy0) + (1.8, 0)$);
            %% X
            \draw (x) -| ($(x) + (0, 0)$) |- (xandy0.input 1);
            
            %Y'

            \draw [line width=0.25mm,   red] (noty.output) -- ([xshift=0cm]noty.output) |- (xandy0.input 2);
              %%W
            \draw (w) -| ($(w) + (0, 0)$) |- (xandy0.input 4);
                
           
            \node[and gate US, draw, rotate=0, logic gate inputs=nnnn] at (2.5, 1*1.5) (xandy1) {};
            \draw (xandy1.output) -- node[above]{\scriptsize $A.\bar C.D$} ($(xandy1) + (1.8, 0)$);
            %% X
            \draw (x) -| ($(x) + (0, 0)$) |- (xandy1.input 1);
            
            %%Z'

            \draw [line width=0.25mm,   red] (notz.output) -- ([xshift=0cm]notz.output) |- (xandy1.input 3);
              %%W
            \draw (w) -| ($(w) + (0, 0)$) |- (xandy1.input 4);
                
           
            \node[and gate US, draw, rotate=0, logic gate inputs=nnnn] at (2.5, 2*1.5) (xandy2) {};
            \draw (xandy2.output) -- node[above]{\scriptsize $\bar A.B.C$} ($(xandy2) + (1.8, 0)$);
            
            %% X'

            \draw  [line width=0.25mm,   red] (notx.output) -- ([xshift=0cm]notx.output) |- (xandy2.input 1);
              
            %% Y
            \draw (y) -| ($(y) + (0, 0)$) |- (xandy2.input 2);
        
            %%Z
            \draw (z) -| ($(z) + (0, 0)$) |- (xandy2.input 3);
                
           
            \node[and gate US, draw, rotate=0, logic gate inputs=nnnn] at (2.5, 3*1.5) (xandy3) {};
            \draw (xandy3.output) -- node[above]{\scriptsize $B.C.\bar D$} ($(xandy3) + (1.8, 0)$);
              
            %% Y
            \draw (y) -| ($(y) + (0, 0)$) |- (xandy3.input 2);
        
            %%Z
            \draw (z) -| ($(z) + (0, 0)$) |- (xandy3.input 3);
        
            %%W

            \draw [line width=0.25mm,   red] (notw.output) -- ([xshift=0cm]notw.output) |- (xandy3.input 4);
          \node[or gate US, draw, rotate=0, logic gate inputs=nnnnn] at (5.5, 4*0.5) (xory) {};


                    \draw (xory.output) -- node[above]{\scriptsize$F$} ($(xory) + (1, 0)$);

\draw (xandy0.output) -- ([xshift=1.40cm]xandy0.output) |- (xory.input 4);

\draw (xandy1.output) -- ([xshift=1.35cm]xandy1.output) |- (xory.input 3);

\draw (xandy2.output) -- ([xshift=1.30cm]xandy2.output) |- (xory.input 2);

\draw (xandy3.output) -- ([xshift=1.35cm]xandy3.output) |- (xory.input 1);

 \end{tikzpicture}

\paragraph{Logigramme} de la fonction\\
            %%\missingfigure[figwidth=6cm]{Logigramme}

 \begin{tikzpicture}

\node (x) at (0, 2*1.5) {$A$};
            \node (y) at (0.5, 2*1.5) {$B$};
            \node (z) at (1, 2*1.5) {$C$};
            \node (w) at (1.5, 2*1.5) {$D$};
            \node[not gate US, draw, rotate=270] at ($(x) + (0.25, -0.3)$) (notx) {};
            \draw (x) -- (notx.input); 
            \node[not gate US, draw, rotate=270] at ($(y) + (0.25, -0.3)$) (noty) {};
            \draw (y) -- (noty.input); 
            \node[not gate US, draw, rotate=270] at ($(z) + (0.25, -0.3)$) (notz) {};
            \draw (z) -- (notz.input);
            \node[not gate US, draw, rotate=270] at ($(w) + (0.25, -0.3)$) (notw) {};
            \draw (w) -- (notw.input);
                
           
            \node[and gate US, draw, rotate=0, logic gate inputs=nnnn] at (2.5, 0*1.5) (xandy0) {};
            \draw (xandy0.output) -- node[above]{\scriptsize $A.\bar B.C$} ($(xandy0) + (1.8, 0)$);
            %% X
            \draw (x) -| ($(x) + (0, 0)$) |- (xandy0.input 1);
            
            %Y'

            \draw [line width=0.25mm,   red] (noty.output) -- ([xshift=0cm]noty.output) |- (xandy0.input 2);
          
            %%Z
            \draw (z) -| ($(z) + (0, 0)$) |- (xandy0.input 3);
                
           
            \node[and gate US, draw, rotate=0, logic gate inputs=nnnn] at (2.5, 1*1.5) (xandy1) {};
            \draw (xandy1.output) -- node[above]{\scriptsize $A.C.\bar D$} ($(xandy1) + (1.8, 0)$);
            %% X
            \draw (x) -| ($(x) + (0, 0)$) |- (xandy1.input 1);
            
            %%Z
            \draw (z) -| ($(z) + (0, 0)$) |- (xandy1.input 3);
        
            %%W

            \draw [line width=0.25mm,   red] (notw.output) -- ([xshift=0cm]notw.output) |- (xandy1.input 4);
          \node[or gate US, draw, rotate=0, logic gate inputs=nnn] at (5.5, 2*0.5) (xory) {};


                    \draw (xory.output) -- node[above]{\scriptsize$F$} ($(xory) + (1, 0)$);

\draw (xandy0.output) -- ([xshift=1.40cm]xandy0.output) |- (xory.input 2);

\draw (xandy1.output) -- ([xshift=1.35cm]xandy1.output) |- (xory.input 1);

 \end{tikzpicture}

\paragraph{Logigramme} de la fonction\\
            %%\missingfigure[figwidth=6cm]{Logigramme}

 \begin{tikzpicture}

\node (x) at (0, 1*1.5) {$A$};
            \node (y) at (0.5, 1*1.5) {$B$};
            \node (z) at (1, 1*1.5) {$C$};
            \node (w) at (1.5, 1*1.5) {$D$};
            \node[not gate US, draw, rotate=270] at ($(x) + (0.25, -0.3)$) (notx) {};
            \draw (x) -- (notx.input); 
            \node[not gate US, draw, rotate=270] at ($(y) + (0.25, -0.3)$) (noty) {};
            \draw (y) -- (noty.input); 
            \node[not gate US, draw, rotate=270] at ($(z) + (0.25, -0.3)$) (notz) {};
            \draw (z) -- (notz.input);
            \node[not gate US, draw, rotate=270] at ($(w) + (0.25, -0.3)$) (notw) {};
            \draw (w) -- (notw.input);
                
           
            \node[and gate US, draw, rotate=0, logic gate inputs=nnnn] at (2.5, 0*1.5) (xandy0) {};
            \draw (xandy0.output) -- node[above]{\scriptsize $A.B.C.D$} ($(xandy0) + (1.8, 0)$);
            %% X
            \draw (x) -| ($(x) + (0, 0)$) |- (xandy0.input 1);
              
            %% Y
            \draw (y) -| ($(y) + (0, 0)$) |- (xandy0.input 2);
        
            %%Z
            \draw (z) -| ($(z) + (0, 0)$) |- (xandy0.input 3);
            %%W
            \draw (w) -| ($(w) + (0, 0)$) |- (xandy0.input 4);
        \node[or gate US, draw, rotate=0, logic gate inputs=nn] at (5.5, 1*0.5) (xory) {};


                    \draw (xory.output) -- node[above]{\scriptsize$F$} ($(xory) + (1, 0)$);

\draw (xandy0.output) -- ([xshift=1.40cm]xandy0.output) |- (xory.input 1);

 \end{tikzpicture}

\pagebreak